testdata/direct_filesys.go
@@ -1,8 +1,0 @@
-package example
-
-import "github.com/tchajed/goose/machine/filesys"
-
-func UsingFs(p string) {
-	filesys.Fs.Create("dir", p) // ERROR unexpected select
-	return
-}
